WIP

Clap/Test/Compiler/Traverse/Foldlm.lean
@@ -1,5 +1,6 @@
 import Lean
 import Clap.Test.Compiler.Traverse.Prelude
+import Clap.Compiler.Wheels
 
 namespace ExampruSym
 
@@ -14,14 +15,33 @@ def sigma (x : ℕ) : Option (ℕ) := do
   let x4 ← share (x2 * x2)
   some (x4 * x)
 
-def sigma_unshared (x : ℕ) : Option (ℕ) := do
+-- | `f x → some x fun X ↦` |
+-- |   `y X` |
+-- | `f x >>= y = X` |
+
+abbrev sigma_unshared (x : ℕ) : Option (ℕ) := do
   let x2 ← some (x + x)
   let x4 ← some (x2 + x2)
   -- let x8 ← some (x4 + x4)
   some (x4 + x)
 
-def testFoldlM : Option ℕ := do
-  let xs ← (List.range 8).foldlM (fun state r ↦ do
+
+/--
+`sym_simp`
+[n = 0 | 0.002266s,
+ n = 1 | 0.002572s,
+ n = 2 | 0.002991s,
+ n = 3 | 0.002793s,
+ n = 4 | 0.003781s,
+ n = 5 | 0.006534s,
+ n = 6 | 0.022153s,
+ n = 7 | 0.089189s,
+ n = 8 | 0.517019s,
+ n = 9 | 2.854253s,
+ n = 10 | 16.538841s]
+-/
+def testFoldlM (k : ℕ) : Option ℕ := do
+  let xs ← (List.range k).foldlM (fun state r ↦ do
     let s0 ← sigma_unshared state[0]
     state.set 0 s0
     ) #v[0, 1, 2]
@@ -29,18 +49,17 @@ def testFoldlM : Option ℕ := do
   return x
 
 def eq_def := sigma_unshared.eq_def
-
+#check Lean.Meta.Sym.mkLambdaFVarsS
 -- set_option trace.Clap.Compile.simp.consiliumMagnum true in
 -- set_option trace.Clap.Compile.simp.proc.vector_foldlM_stagger true in
 -- set_option Clap.traversalDbg true in
-set_option trace.Clap.Compile.dbg true in
--- set_option trace.Clap.Compile.simp.proc.beta true in
-set_option maxRecDepth 100000 in
-set_option maxHeartbeats 0 in
-#eval runOptionNTestByName ``testFoldlM (extraPasses := mkMethods #[
-  (``eq_def, .Pre)
-] (atMostOnce := false))
-
+-- set_option trace.Clap.Compile.dbg true in
+-- -- set_option trace.Clap.Compile.simp.proc.beta true in
+-- set_option maxRecDepth 100000 in
+-- set_option maxHeartbeats 0 in
+-- #eval runOptionNTestByName ``testFoldlM (extraPasses := mkMethods #[
+--   (``eq_def, .Pre)
+-- ] (atMostOnce := false))
 
 -- THE PLAN
 -- use sigma unshared - done
@@ -49,9 +68,48 @@ set_option maxHeartbeats 0 in
 -- reset its log in the debug state at the end of each consiliumMagnum iteration - done
 -- rejoice - todo
 
-
-
 open Lean Meta Elab Tactic
+
+def bench_sym : Lean.MetaM Unit := do
+  let rewrite ← Sym.mkSimprocFor #[
+    ``testFoldlM.eq_def,
+    ``sigma_unshared.eq_def,
+    ``bind_assoc,
+    ``Option.bind_eq_bind,
+    ``Option.bind_some,
+    ``List.range.eq_def,
+    ``List.range.loop.eq_def,
+    ``List.foldlM_cons,
+    ``Vector.getElem_mk,
+    ``List.getElem_toArray,
+    ``List.getElem_cons_zero,
+    ``Vector.set_mk,
+    ``List.set_toArray,
+    ``List.set_cons_zero,
+    ``List.foldlM_nil,
+    ``Option.pure_def,
+    ``Option.bind_fun_some
+  ]
+  let methods : Sym.Simp.Methods := {
+    pre  := Sym.Simp.simpControl
+    post := Sym.Simp.evalGround >> rewrite
+  }
+  let inputSizes : Array Nat := Array.range 11
+  let results ← inputSizes.mapM fun inputSize ↦ do
+    Sym.SymM.run do
+      let expr ← Clap.Compiler.Simp.preprocessExpr
+        (((←getEnv).find? ``testFoldlM).get!.value!.beta #[mkNatLit inputSize])
+      let (_, time) ← Clap.Dbg.timeS (Sym.simp expr methods)
+      return time
+      -- logInfo m!"Sym.simp took: {time}s"
+      -- logInfo m!"res: {res.getResultExpr expr}"
+  let results := results.zip inputSizes
+  let results :=
+    results.map fun (time, n) ↦ s!"n = {n} | {time}s"
+  logInfo m!"{results}"
+
+-- set_option maxHeartbeats 0 in
+-- #eval bench
 
 elab "sym_simp" "[" declNames:ident,* "]" : tactic => do
   let rewrite ← Sym.mkSimprocFor (← declNames.getElems.mapM fun s => realizeGlobalConstNoOverload s.raw) Sym.Simp.dischargeSimpSelf
@@ -61,9 +119,18 @@ elab "sym_simp" "[" declNames:ident,* "]" : tactic => do
   }
   liftMetaTactic1 fun mvarId => Sym.SymM.run do
     let mvarId ← Sym.preprocessMVar mvarId
-    (← Sym.simpGoal mvarId methods).toOption
+    let (res, time) ← Clap.Dbg.timeS (Sym.simpGoal mvarId methods)
+    logInfo m!"Sym.simp took: {time}s"
+    res.toOption
 
-example : testFoldlM = sorry := by
+-- 1 = 0.002309s
+-- 2 = 0.003176s
+-- 4 = 0.004275s
+-- 6 = 0.018588s
+-- 8 = 0.421613s
+-- 12 = 
+-- set_option maxHeartbeats 0 in
+example : testFoldlM = testFoldlM := by
   sym_simp [
     testFoldlM.eq_def,
     sigma_unshared.eq_def,
